fstar/treedem/MLS.TreeDEM.Message.Framing.fst
@@ -139,17 +139,21 @@ let message_to_sender_data_aad #bytes #bl content =
     content_type = content.content.content_type;
   } <: sender_data_aad_nt bytes)
 
-val decrypt_sender_data: #bytes:Type0 -> {|crypto_bytes bytes|} -> sender_data_aad_nt bytes -> ciphertext_sample:bytes -> sender_data_secret:bytes -> encrypted_sender_data:bytes -> result (sender_data_nt bytes)
-let decrypt_sender_data #bytes #cb ad ciphertext_sample sender_data_secret encrypted_sender_data =
+val sender_data_key_nonce: #bytes:Type0 -> {|crypto_bytes bytes|} -> ciphertext_sample:bytes -> sender_data_secret:bytes -> result (lbytes bytes (aead_key_length #bytes) & lbytes bytes (aead_nonce_length #bytes))
+let sender_data_key_nonce #bytes #cb ciphertext_sample sender_data_secret =
   let? sender_data_key = expand_with_label sender_data_secret (string_to_bytes #bytes "key") ciphertext_sample (aead_key_length #bytes) in
   let? sender_data_nonce = expand_with_label sender_data_secret (string_to_bytes #bytes "nonce") ciphertext_sample (aead_nonce_length #bytes) in
+  return (sender_data_key, sender_data_nonce)
+
+val decrypt_sender_data: #bytes:Type0 -> {|crypto_bytes bytes|} -> sender_data_aad_nt bytes -> ciphertext_sample:bytes -> sender_data_secret:bytes -> encrypted_sender_data:bytes -> result (sender_data_nt bytes)
+let decrypt_sender_data #bytes #cb ad ciphertext_sample sender_data_secret encrypted_sender_data =
+  let? (sender_data_key, sender_data_nonce) = sender_data_key_nonce sender_data_secret  ciphertext_sample in
   let? sender_data = aead_decrypt sender_data_key sender_data_nonce (serialize (sender_data_aad_nt bytes) ad) encrypted_sender_data in
   from_option "decrypt_sender_data: malformed sender data" (parse (sender_data_nt bytes) sender_data)
 
 val encrypt_sender_data: #bytes:Type0 -> {|crypto_bytes bytes|} -> sender_data_aad_nt bytes -> ciphertext_sample:bytes -> sender_data_secret:bytes -> sender_data_nt bytes -> result bytes
 let encrypt_sender_data #bytes #cb ad ciphertext_sample sender_data_secret sender_data =
-  let? sender_data_key = expand_with_label sender_data_secret (string_to_bytes #bytes "key") ciphertext_sample (aead_key_length #bytes) in
-  let? sender_data_nonce = expand_with_label sender_data_secret (string_to_bytes #bytes "nonce") ciphertext_sample (aead_nonce_length #bytes) in
+  let? (sender_data_key, sender_data_nonce) = sender_data_key_nonce sender_data_secret  ciphertext_sample in
   aead_encrypt sender_data_key sender_data_nonce (serialize (sender_data_aad_nt bytes) ad) (serialize (sender_data_nt bytes) sender_data)
 
 // Used in decryption
